vlsm.v
@@ -23,7 +23,10 @@ Class VLSM (message : Type) :=
   ; label_inhabited : inhabited label
   ; transition : label -> state * option proto_message -> state * option proto_message
   ; valid : label -> state * option proto_message -> Prop
-  ; valid_decidable : forall l som, {valid l som} + {~valid l som}
+  }.
+
+Class VLSM_vdecidable (message : Type) `{M : VLSM message} :=
+  { valid_decidable : forall l som, {valid l som} + {~valid l som} 
   }.
 
 (* 2.2.2 VLSM protocol states and protocol messages *)
